stdlib/iterator/src/adapters/take.rs
@@ -1,0 +1,42 @@
+use crate::traits::iterator::Iterator;
+
+#[rr::export_as(core::iter::adapters::Take)]
+#[rr::refined_by("(it, n)" : "(_ * nat)")]
+pub struct Take<I> {
+    #[rr::field("it")]
+    iter: I,
+    #[rr::field("Z.of_nat n")]
+    n: usize,
+}
+
+#[rr::export_as(core::iter::adapters::Take)]
+impl<I> Take<I> {
+    #[rr::returns("(iter, Z.to_nat n)")]
+    pub fn new(iter: I, n: usize) -> Take<I> {
+        Take { iter, n }
+    }
+}
+
+
+#[rr::instantiate("Params" := "{MI::Params}")]
+#[rr::instantiate("Inv" := "λ π p s, {MI::Inv} π p s.1")]
+// TODO: could also unify the decide branches, but that depends a bit on how easily we can simplify seq to [] in that case
+#[rr::instantiate("Next" := "(λ π p_inner s1 e s2, 
+        if_iNone e (
+            (⌜s1.2 = 0%nat⌝ ∗ True) ∨ (⌜s1.2 ≠ 0%nat⌝ ∗ ⌜s2.2 = (s1.2 - 1)%nat⌝ ∗ {MI::Next} π p_inner s1.1 None s2.1)) ∗ 
+        if_iSome e (λ e, ⌜s1.2 > 0%nat⌝ ∗ ⌜s2.2 = (s1.2 - 1)%nat⌝ ∗ {MI::Next} π p_inner s1.1 (Some e) s2.1))%I")]
+impl<MI> Iterator for Take<MI>
+where
+    MI: Iterator,
+{
+    type Item = <MI as Iterator>::Item;
+
+    fn next(&mut self) -> Option<<MI as Iterator>::Item> {
+        if self.n != 0 {
+            self.n -= 1;
+            self.iter.next()
+        } else {
+            None
+        }
+    }
+}
