stdlib/iterator/output/iterator/proofs/proof_adapters_skip_SkipMIastraits_iterator_Iterator_next.v
@@ -1,0 +1,51 @@
+From caesium Require Import lang notation.
+From refinedrust Require Import typing shims.
+From rrstd.iterator.iterator.generated Require Import generated_code_iterator generated_specs_iterator generated_template_adapters_skip_SkipMIastraits_iterator_Iterator_next.
+
+Set Default Proof Using "Type".
+
+Section proof.
+Context `{RRGS : !refinedrustGS Σ}.
+
+Lemma adapters_skip_SkipMIastraits_iterator_Iterator_next_proof (π : thread_id) :
+  adapters_skip_SkipMIastraits_iterator_Iterator_next_lemma π.
+Proof.
+  adapters_skip_SkipMIastraits_iterator_Iterator_next_prelude.
+
+  rep <-! liRStep; liShow.
+  { (* unfold invariant *)
+    iRename select (traits_iterator_Iterator_Inv _ _ _ _) into "Hinv".
+    iEval (rewrite /traits_iterator_Iterator_Inv/=) in "Hinv".
+    rep <-! liRStep; liShow.
+    rep <- 20 liRStep; liShow.
+    { liRStep; liShow. liRStep; liShow.
+      liRStep; liShow. liRStep; liShow.
+      liRStep; liShow. liInst Hevar_s2_inner x'.
+      iEval (rewrite /traits_iterator_Iterator_Inv/=).
+      rep liRStep; liShow. }
+    { rep liRStep; liShow.
+      liInst Hevar_seq x'1. liInst Hevar_s2_inner x'.
+      rep <- 1 liRStep; liShow.
+      iEval (rewrite /traits_iterator_Iterator_Inv/=).
+      rep liRStep; liShow. } }
+  rep <-! liRStep; liShow.
+  { (* unfold invariant *)
+    iRename select (traits_iterator_Iterator_Inv _ _ _ _) into "Hinv".
+    iEval (rewrite /traits_iterator_Iterator_Inv/=) in "Hinv".
+    rep <-! liRStep; liShow.
+    rep <- 1 liRStep; liShow.
+    { iEval (rewrite /traits_iterator_Iterator_Inv/=).
+      rep liRStep; liShow.
+      liInst Hevar_seq [].
+      rep liRStep; liShow. }
+    { iEval (rewrite /traits_iterator_Iterator_Inv/=).
+      rep liRStep; liShow.
+      liInst Hevar_seq [].
+      rep liRStep; liShow. } }
+
+  all: print_remaining_goal.
+  Unshelve. all: sidecond_solver.
+  Unshelve. all: sidecond_hammer.
+  Unshelve. all: print_remaining_sidecond.
+Qed.
+End proof.
