stdlib/iterator/output/iterator/proofs/proof_traits_iterator_Iterator_nth.v
@@ -1,0 +1,37 @@
+From caesium Require Import lang notation.
+From refinedrust Require Import typing shims.
+From rrstd.iterator.iterator.generated Require Import generated_code_iterator generated_specs_iterator generated_template_traits_iterator_Iterator_nth.
+
+Set Default Proof Using "Type".
+
+Section proof.
+Context `{RRGS : !refinedrustGS Σ}.
+
+Lemma traits_iterator_Iterator_nth_proof (π : thread_id) :
+  traits_iterator_Iterator_nth_lemma π.
+Proof.
+  traits_iterator_Iterator_nth_prelude.
+
+  rep <-! liRStep; liShow.
+  { rep liRStep; liShow.
+    liInst Hevar_x0 seq. 
+    liInst Hevar_x1 x1.
+    rep liRStep; liShow.
+    liInst Hevar_x2 x'.
+    rep liRStep; liShow. }
+  { rep liRStep; liShow.
+    liInst Hevar_seq (seq ++ [y]).
+    rep liRStep; liShow. }
+  { rep liRStep; liShow.
+    liInst Hevar_x0 seq. 
+    liInst Hevar_x1 x1.
+    rep liRStep; liShow.
+    liInst Hevar_x2 x'.
+    rep liRStep; liShow. }
+
+  all: print_remaining_goal.
+  Unshelve. all: sidecond_solver.
+  Unshelve. all: sidecond_hammer.
+  Unshelve. all: print_remaining_sidecond.
+Qed.
+End proof.
